\section{Quadratic equations}
\begin{outline}

\0
\subsection{Expanding expressions}
	\1 Necessary knowledge
		\2 Like terms
			\3 Like terms have the same pronumeral part. They can be collected (added and subtracted) to form a single term.
				\[7x - 11x = -4x\]
				\[4a^2b - 7ba^2 = -3a^2b\]
		\2 The distributive law
			\3 The distributive law is used to expand brackets.
				\[a(b + c) = ab + ac \text{ and } a(b - c) = ab - ac\]
				\[(a + b)(c + d) = ac + ad + bc + bd\]
	 	 	$(a + b)(c + d)$ is a binomial product because each expression within the parenthesis has two terms.
		\2 Perfect squares
	 	 	\[(a + b)^2 = (a + b)(c + d) = a^2 + 2ab + b^2\]
	 	 	\[(a - b)^2 = (a - b)(a - b) = a^2 - 2ab + b^2\]
		\2 Difference of perfect squares
	 	 	\[(a + b)(a - b) = a^2 - b^2\]
	\1 Expanding simple expressions
	\1 Expanding binomial products, perfect squares and difference of perfect squares
	\1 Expanding more binomial products

\0
\subsection{Factorising expressions}

\0
\subsection{Factorising trinomials of the form $x^2 + bx + c$}

\0
\subsection{Factorising quadratic trinomials of the form $ax^2 + bx + c$}

\0
\subsection{Factorising by completing the square}

\0
\subsection{Solving quadratic equations}

\0
\subsection{Applications of quadratics}

\0
\subsection{Solving quadratic equations by completing the square}

\0
\subsection{The quadratic formula}

\end{outline}
